.

theories/Logic/ConstructiveDomainTheory.v
@@ -1,3 +1,4 @@
+Require Import Coq.Lists.List.
 Require Import Coq.Program.Basics.
 Require Import DschingisKhan.Prelude.PreludeInit.
 Require Import DschingisKhan.Prelude.PreludeMath.
@@ -9,7 +10,7 @@ Module BasicCoLaTheory.
 
   Local Existing Instances pair_isPoset arrow_isPoset.
 
-  Global Hint Constructors _image : poset_hints.
+  Global Hint Constructors _image _finite : poset_hints.
 
   Definition getInfimumOf_inCoLa {D : Type} {requiresPoset : isPoset D} {requiresCoLa : isCoLa D} (X : ensemble D) : {inf_X : D | isInfimumOf inf_X X} :=
     let inf_X : D := proj1_sig (getSupremumOf_inCoLa (LowerBoundsOf X)) in
@@ -42,14 +43,14 @@ Module BasicCoLaTheory.
     transitivity (proj1_sig f x'); [eapply (proj2_sig f) | eapply supOfMonotonicMaps_proj2_sig with (x := x')]; eauto with *.
   Qed.
 
-  Definition supremum_m {dom : Type} {cod : Type} {dom_isPoset : isPoset dom} {cod_isPoset : isPoset cod} {dom_isCoLa : isCoLa dom} {cod_isCoLa : isCoLa cod} (fs : ensemble ⟬ dom ⟶ cod ⟭) : ⟬ dom ⟶ cod ⟭ :=
+  Definition SupOfMonotonicMaps {dom : Type} {cod : Type} {dom_isPoset : isPoset dom} {cod_isPoset : isPoset cod} {dom_isCoLa : isCoLa dom} {cod_isCoLa : isCoLa cod} (fs : ensemble ⟬ dom ⟶ cod ⟭) : ⟬ dom ⟶ cod ⟭ :=
     @exist (dom -> cod) isMonotonicMap (supOfMonotonicMaps fs) (supOfMonotonicMaps_isMonotonicMap fs)
   .
 
-  Lemma supremum_m_isSupremum {dom : Type} {cod : Type} {dom_isPoset : isPoset dom} {cod_isPoset : isPoset cod} {dom_isCoLa : isCoLa dom} {cod_isCoLa : isCoLa cod}
-    : forall fs : ensemble ⟬ dom ⟶ cod ⟭, isSupremumOf (supremum_m fs) fs.
+  Lemma SupOfMonotonicMaps_isSupremum {dom : Type} {cod : Type} {dom_isPoset : isPoset dom} {cod_isPoset : isPoset cod} {dom_isCoLa : isCoLa dom} {cod_isCoLa : isCoLa cod}
+    : forall fs : ensemble ⟬ dom ⟶ cod ⟭, isSupremumOf (SupOfMonotonicMaps fs) fs.
   Proof with eauto with *.
-    unfold supremum_m; intros fs f. split; intros ?; desnw.
+    unfold SupOfMonotonicMaps; intros fs f. split; intros ?; desnw.
     - intros f_i f_i_in. rewrite <- SUPREMUM_LE_UPPER_BOUND.
       intros x. simpl. eapply supOfMonotonicMaps_proj2_sig with (x := x)...
     - intros x. simpl. eapply supOfMonotonicMaps_proj2_sig with (x := x).
@@ -58,8 +59,86 @@ Module BasicCoLaTheory.
   Qed.
 
   Local Instance MonotonicMaps_isCoLa (dom : Type) (cod : Type) {dom_isPoset : isPoset dom} {cod_isPoset : isPoset cod} {dom_isCoLa : isCoLa dom} {cod_isCoLa : isCoLa cod} : isCoLa ⟬ dom ⟶ cod ⟭ :=
-    fun fs : ensemble ⟬ dom ⟶ cod ⟭ => @exist ⟬ dom ⟶ cod ⟭ (fun sup_fs : ⟬ dom ⟶ cod ⟭ => isSupremumOf sup_fs fs) (supremum_m fs) (supremum_m_isSupremum fs)
+    fun fs : ensemble ⟬ dom ⟶ cod ⟭ => @exist ⟬ dom ⟶ cod ⟭ (fun sup_fs : ⟬ dom ⟶ cod ⟭ => isSupremumOf sup_fs fs) (SupOfMonotonicMaps fs) (SupOfMonotonicMaps_isSupremum fs)
   .
+
+  Lemma getLeastFixedPoint_inCoLa {D : Type} {D_isPoset : isPoset D} {D_isCoLa : isCoLa D} (f : D -> D)
+    (f_isMonotonic : isMonotonicMap f)
+    : {lfp_f : D | isInfimumOf lfp_f (PrefixedPoints f) /\ isLeastFixedPointOf lfp_f f}.
+  Proof.
+    assert (IS_INFIMUM : isInfimumOf (proj1_sig (getInfimumOf_inCoLa (PrefixedPoints f))) (PrefixedPoints f)) by exact (proj2_sig (getInfimumOf_inCoLa (PrefixedPoints f))).
+    exists (proj1_sig (getInfimumOf_inCoLa (PrefixedPoints f))). split.
+    - exact (IS_INFIMUM).
+    - eapply theLeastFixedPointOfMonotonicMap.
+      + exact (f_isMonotonic).
+      + exact (IS_INFIMUM).
+  Defined.
+
+  Lemma getGreatestFixedPoint_inCoLa {D : Type} {D_isPoset : isPoset D} {D_isCoLa : isCoLa D} (f : D -> D)
+    (f_isMonotonic : isMonotonicMap f)
+    : {gfp_f : D | isSupremumOf gfp_f (PostfixedPoints f) /\ isGreatestFixedPointOf gfp_f f}.
+  Proof.
+    assert (IS_SUPREMUM : isSupremumOf (proj1_sig (getSupremumOf_inCoLa (PostfixedPoints f))) (PostfixedPoints f)) by exact (proj2_sig (getSupremumOf_inCoLa (PostfixedPoints f))).
+    exists (proj1_sig (getSupremumOf_inCoLa (PostfixedPoints f))). split.
+    - exact (IS_SUPREMUM).
+    - eapply theGreatestFixedPointOfMonotonicMap.
+      + exact (f_isMonotonic).
+      + exact (IS_SUPREMUM).
+  Defined.
+
+  Definition nu {D : Type} {D_isPoset : isPoset D} {D_isCoLa : isCoLa D (requiresPoset := D_isPoset)} (f : ⟬ D ⟶ D ⟭) : {gfp_f : D | isGreatestFixedPointOf gfp_f (proj1_sig f)} :=
+    let nu_proj1_sig : D := proj1_sig (getSupremumOf_inCoLa (PostfixedPoints (proj1_sig f))) in
+    let IS_SUPREMUM : isSupremumOf nu_proj1_sig (PostfixedPoints (proj1_sig f)) := proj2_sig (getSupremumOf_inCoLa (PostfixedPoints (proj1_sig f))) in
+    @exist D (fun gfp_f : D => isGreatestFixedPointOf gfp_f (proj1_sig f)) nu_proj1_sig (theGreatestFixedPointOfMonotonicMap (proj1_sig f) nu_proj1_sig (proj2_sig f) IS_SUPREMUM)
+  .
+
+  Corollary nu_isSupremumOf_PostfixedPoints {D : Type} {D_isPoset : isPoset D} {D_isCoLa : isCoLa D (requiresPoset := D_isPoset)} (f : ⟬ D ⟶ D ⟭)
+    : isSupremumOf (proj1_sig (nu f)) (PostfixedPoints (proj1_sig f)).
+  Proof. exact (proj2_sig (getSupremumOf_inCoLa (PostfixedPoints (proj1_sig f)))). Qed.
+
+  Section PACO_METATHEORY.
+
+  Import ListNotations MathNotations.
+
+  Class ExtraColaMethods (D : Type) {requiresPoset : isPoset D} : Type :=
+    { cola_union (d_left : D) (d_right : D) : D
+    ; cola_empty : D
+    ; cola_union_spec (d_left : D) (d_right : D)
+      : isSupremumOf (cola_union d_left d_right) (finite [d_left; d_right])
+    ; cola_empty_spec
+      : isSupremumOf (cola_empty) (empty)
+    }
+  .
+
+  Context {D : Type} {requiresPoset : isPoset D}.
+
+  Lemma le_cola_union_introl {hasExtraColaMethods : ExtraColaMethods D} (x1 : D) (x2 : D)
+    : x1 =< cola_union x1 x2.
+  Proof. eapply cola_union_spec; eauto with *. Qed.
+
+  Lemma le_cola_union_intror {hasExtraColaMethods : ExtraColaMethods D} (x1 : D) (x2 : D)
+    : x2 =< cola_union x1 x2.
+  Proof. eapply cola_union_spec; eauto with *. Qed.
+
+  Lemma cola_union_le_iff {hasExtraColaMethods : ExtraColaMethods D} (x1 : D) (x2 : D) (x : D)
+    : cola_union x1 x2 =< x <-> (x1 =< x /\ x2 =< x).
+  Proof with eauto with *.
+    split.
+    - intros ?; split; eapply cola_union_spec...
+    - intros [x1_le_x x2_le_x]. eapply cola_union_spec.
+      intros d d_in. apply in_finite_iff in d_in.
+      destruct d_in as [d_eq_x1 | [d_eq_x2 | []]]; subst d...
+  Qed.
+
+  Lemma cola_empty_le_intro {hasExtraColaMethods : ExtraColaMethods D} (x : D)
+    : cola_empty =< x.
+  Proof.
+    eapply cola_empty_spec.
+    intros d d_in. apply in_empty_iff in d_in.
+    destruct d_in as [].
+  Qed.
+
+  End PACO_METATHEORY.
 
 End BasicCoLaTheory.
 
